tactics.v
@@ -1,0 +1,227 @@
+From mathcomp Require Import ssreflect.
+From stdpp Require Import gmap.
+From iris.algebra Require Import agree auth gset gmap.
+From iris.base_logic.lib Require Import invariants.
+From iris.heap_lang Require Import notation proofmode.
+From iris.proofmode Require Import base environments.
+From crypto Require Import lib basic term crypto1 primitives.
+Import bi.
+Import env_notations.
+
+Section Proofs.
+
+Context `{!heapG Σ, !resG Σ}.
+
+Implicit Types E : coPset.
+Implicit Types l : loc.
+Implicit Types lvl : level.
+Implicit Types t : term.
+Implicit Types v : val.
+Implicit Types Φ : prodO locO termO -n> iPropO Σ.
+Implicit Types Ψ : val → iProp Σ.
+
+Lemma tac_twp_untag Γ E K n t Ψ :
+  (∀ t', t = Spec.tag n t' →
+         envs_entails Γ (WP fill K (Val (repr (Some t'))) @ E [{ Ψ }])) →
+  (Spec.untag n t = None →
+   envs_entails Γ (WP fill K (Val NONEV) @ E [{ Ψ }])) →
+  envs_entails Γ (WP fill K (untag n t) @ E [{ Ψ }]).
+Proof.
+rewrite envs_entails_eq => HSome HNone.
+rewrite -twp_bind -twp_untag.
+case e: Spec.untag => [t'|].
+- by move/Spec.untagK in e; apply: HSome.
+- exact: HNone.
+Qed.
+
+Lemma tac_wp_untag Γ E K n t Ψ :
+  (∀ t', t = Spec.tag n t' →
+         envs_entails Γ (WP fill K (Val (repr (Some t'))) @ E {{ Ψ }})) →
+  (Spec.untag n t = None →
+   envs_entails Γ (WP fill K (Val NONEV) @ E {{ Ψ }})) →
+  envs_entails Γ (WP fill K (untag n t) @ E {{ Ψ }}).
+Proof.
+rewrite envs_entails_eq => HSome HNone.
+rewrite -wp_bind -wp_untag.
+case e: Spec.untag => [t'|].
+- by move/Spec.untagK in e; apply: HSome.
+- exact: HNone.
+Qed.
+
+(* TODO: Generalize to symmetric encryption *)
+Lemma tac_twp_dec Γ E K k t Ψ :
+  (∀ t', t = TEnc true k t' →
+         envs_entails Γ (WP fill K (Val (SOMEV t')) @ E [{ Ψ }])) →
+  (Spec.dec (TKey KADec k) t = None →
+   envs_entails Γ (WP fill K (Val NONEV) @ E [{ Ψ }])) →
+  envs_entails Γ (WP fill K (dec (TKey KADec k) t) @ E [{ Ψ }]).
+Proof.
+rewrite envs_entails_eq => HSome HNone.
+rewrite -twp_bind -twp_dec.
+case: t HSome HNone; eauto.
+case; eauto => k' /=.
+by case: decide => [<-|]; eauto.
+Qed.
+
+Lemma tac_wp_dec Γ E K k t Ψ :
+  (∀ t', t = TEnc true k t' →
+         envs_entails Γ (WP fill K (Val (SOMEV t')) @ E {{ Ψ }})) →
+  (Spec.dec (TKey KADec k) t = None →
+   envs_entails Γ (WP fill K (Val NONEV) @ E {{ Ψ }})) →
+  envs_entails Γ (WP fill K (dec (TKey KADec k) t) @ E {{ Ψ }}).
+Proof.
+rewrite envs_entails_eq => HSome HNone.
+rewrite -wp_bind -wp_dec.
+case: t HSome HNone; eauto.
+case; eauto => k' /=.
+by case: decide => [<-|]; eauto.
+Qed.
+
+Lemma tac_twp_list_of_term Γ E K t Ψ :
+  (∀ ts, t = Spec.of_list ts →
+         envs_entails Γ (WP fill K (Val (SOMEV (repr ts))) @ E [{ Ψ }])) →
+  (Spec.to_list t = None →
+   envs_entails Γ (WP fill K NONEV @ E [{ Ψ }])) →
+  envs_entails Γ (WP fill K (list_of_term t) @ E [{ Ψ }]).
+Proof.
+rewrite envs_entails_eq => HSome HNone.
+rewrite -twp_bind -twp_list_of_term.
+case e: Spec.to_list => [ts|]; eauto.
+move/Spec.to_listK in e; subst t; eauto.
+Qed.
+
+Lemma tac_wp_list_of_term Γ E K t Ψ :
+  (∀ ts, t = Spec.of_list ts →
+         envs_entails Γ (WP fill K (Val (SOMEV (repr ts))) @ E {{ Ψ }})) →
+  (Spec.to_list t = None →
+   envs_entails Γ (WP fill K NONEV @ E {{ Ψ }})) →
+  envs_entails Γ (WP fill K (list_of_term t) @ E {{ Ψ }}).
+Proof.
+rewrite envs_entails_eq => HSome HNone.
+rewrite -wp_bind -wp_list_of_term.
+case e: Spec.to_list => [ts|]; eauto.
+move/Spec.to_listK in e; subst t; eauto.
+Qed.
+
+(* TODO:
+- Generalize to other instances of Repr
+- rename get_list -> lookup *)
+Lemma tac_twp_lookup Γ E K ts (n : Z) Ψ :
+  (0 <= n)%Z →
+  (∀ t, (ts !! Z.to_nat n)%stdpp = Some t →
+        envs_entails Γ (WP fill K (Val (SOMEV t)) @ E [{ Ψ }])) →
+  ((ts !! Z.to_nat n)%stdpp = None →
+   envs_entails Γ (WP fill K (Val NONEV) @ E [{ Ψ }])) →
+  envs_entails Γ (WP fill K (repr ts !! #n)%E @ E [{ Ψ }]).
+Proof.
+move=> npos; rewrite -[in #n](Z2Nat.id n) //.
+move: (Z.to_nat _)=> {npos} n.
+rewrite envs_entails_eq => HSome HNone.
+rewrite -twp_bind -twp_get_list.
+by case e: (_ !! n)%stdpp => [t|]; eauto.
+Qed.
+
+Lemma tac_wp_lookup Γ E K ts (n : Z) Ψ :
+  (0 <= n)%Z →
+  (∀ t, (ts !! Z.to_nat n)%stdpp = Some t →
+        envs_entails Γ (WP fill K (Val (SOMEV t)) @ E {{ Ψ }})) →
+  ((ts !! Z.to_nat n)%stdpp = None →
+   envs_entails Γ (WP fill K (Val NONEV) @ E {{ Ψ }})) →
+  envs_entails Γ (WP fill K (repr ts !! #n)%E @ E {{ Ψ }}).
+Proof.
+move=> npos; rewrite -[in #n](Z2Nat.id n) //.
+move: (Z.to_nat _)=> {npos} n.
+rewrite envs_entails_eq => HSome HNone.
+rewrite -wp_bind -wp_get_list.
+by case e: (_ !! n)%stdpp => [t|]; eauto.
+Qed.
+
+Lemma tac_wp_eq_term Γ E K t1 t2 Ψ :
+  (t1 = t2 →
+   envs_entails Γ (WP fill K (Val #true) @ E {{ Ψ }})) →
+  (t1 ≠ t2 →
+   envs_entails Γ (WP fill K (Val #false) @ E {{ Ψ }})) →
+  envs_entails Γ (WP fill K (eq_term t1 t2) @ E {{ Ψ }}).
+Proof.
+rewrite envs_entails_eq => HSome HNone.
+rewrite -wp_bind -wp_eq_term.
+by case: bool_decide_reflect; eauto.
+Qed.
+
+End Proofs.
+
+Tactic Notation "wp_list" open_constr(t) :=
+  wp_pures; wp_bind (_ :: _)%E; iApply (wp_list t).
+
+Tactic Notation "wp_term_of_list" :=
+  wp_pures; wp_bind (term_of_list _); iApply wp_term_of_list.
+
+Tactic Notation "wp_tag" :=
+  wp_pures; wp_bind (tag _ _); iApply wp_tag.
+
+Tactic Notation "wp_enc" :=
+  wp_pures; wp_bind (enc _ _); iApply wp_enc.
+
+Tactic Notation "wp_dec_eq" ident(t) ident(H) :=
+  wp_pures;
+  lazymatch goal with
+  | |- envs_entails _ (wp ?s ?E ?e ?Q) =>
+    reshape_expr e ltac:(fun K e' =>
+      first
+        [eapply (tac_wp_dec _ _ K _ _);
+         [intros t H|intros H];
+         wp_finish
+        |fail 1 "wp_dec: Cannot decode"])
+  end.
+
+Tactic Notation "wp_dec" ident(t) :=
+  let tf := fresh "tf" in
+  let H := fresh "H" in
+  wp_dec_eq tf H; [
+    first [revert t tf H; intros _ t ->
+          |revert tf H; intros _ t ->
+          |revert tf H; intros t _]
+  | clear H].
+
+Tactic Notation "wp_list_of_term_eq" ident(t) ident(H) :=
+  wp_pures;
+  lazymatch goal with
+  | |- envs_entails _ (wp ?s ?E ?e ?Q) =>
+    reshape_expr e ltac:(fun K e' =>
+      first
+        [eapply (tac_wp_list_of_term _ _ K _ _);
+         [intros t H|intros H];
+         wp_finish
+        |fail 1 "wp_dec: Cannot decode"])
+  end.
+
+Tactic Notation "wp_list_of_term" ident(t) :=
+  let tf := fresh "tf" in
+  let H := fresh "H" in
+  wp_list_of_term_eq tf H; [
+    first [revert t tf H; intros _ t ->
+          |revert tf H; intros _ t ->
+          |revert tf H; intros t _]
+  | clear H].
+
+Tactic Notation "wp_lookup" ident(t) ident(H) :=
+  wp_pures;
+  lazymatch goal with
+  | |- envs_entails _ (wp ?s ?E ?e ?Q) =>
+    reshape_expr e ltac:(fun K e' =>
+      first
+        [eapply (tac_wp_lookup _ _ K _ _);
+         [lia|intros t H|intros H];
+         wp_finish
+        |fail 1 "wp_lookup: Cannot decode"])
+  end.
+
+Tactic Notation "wp_eq_term" ident(H) :=
+  wp_pures;
+  lazymatch goal with
+  | |- envs_entails _ (wp ?s ?E ?e ?Q) =>
+    reshape_expr e ltac:(fun K e' =>
+      first
+        [eapply (tac_wp_eq_term _ _ K _ _); intros H; wp_finish
+        |fail 1 "wp_eq_term: Cannot decode"])
+  end.
